q

while_not_b.ec
@@ -3,64 +3,67 @@ pragma Goals:printall.
 require import AllCore DBool.
 
 require import Int.
-op myd : int distr.
+
+type rt.
+
+op myd : rt distr.
+op MyP : rt -> bool.
 
 module M = {
   var c : int
-  proc whp(s : int, e : int, b : bool, r : int) = {
+  proc whp(s : int, e : int, r : rt) = {
     c <- s;
-    while(c <= e /\ !b ){
+    while(c <= e /\ !MyP r){
      r <$ myd;
-     b <$ {0,1};
      c <- c + 1;
     }
-    return (r,b);
+    return r;
   }
 
-  proc whp_if_end(s : int, e : int, b : bool, r : int) = {
-    (r,b) <- whp(s,e,b,r);     
-    if(c <= e + 1 /\ !b){
-      r <$ myd;
-      b <$ {0,1};
+  proc whp_if_end(s : int, e : int, r : rt) = {
+    var ri : rt;
+    ri <- whp(s,e,r);     
+    if(c <= e + 1 /\ !MyP ri){
+      ri <$ myd;
       c <- c + 1;
     }
-    return (r,b);
+    return ri;
   }
 }.
 
 
 lemma whp_split_if_end :  
-  equiv[ M.whp ~ M.whp_if_end : ={s,b,r} /\ e{1} - 1 = e{2}
+  equiv[ M.whp ~ M.whp_if_end : ={s,r} /\ e{1} - 1 = e{2}
         ==> ={res,M.c} ].
 proof. proc.
 inline*. sp. 
 splitwhile{1} 1 : M.c  <= (e - 1) .
-seq  1 1 : (={M.c} /\ b{1} = b0{2} /\ r{1} = r0{2} /\ e0{2} = e{2}
-   /\ e{1} - 1 = e0{2} /\ (!b{1} => (e{1} - 1) < M.c{1} )).
-while (={M.c} /\ b{1} = b0{2} /\ r{1} = r0{2} /\ e0{2} = e{2}
+seq  1 1 : (={M.c} /\ r{1} = r0{2} /\ e0{2} = e{2}
+   /\ e{1} - 1 = e0{2} /\ (!MyP r{1} => (e{1} - 1) < M.c{1} )).
+while (={M.c} /\ r{1} = r0{2} /\ e0{2} = e{2}
    /\ e{1} - 1 = e0{2} ).
-wp. rnd. rnd. skip. progress. smt.  skip. progress. smt. smt.
+wp. rnd. skip. progress. smt.  skip. progress. smt. smt.
 sp. simplify.
-case (b{1}).
+case (MyP r{1}).
 rcondf {1} 1. progress. skip. smt.
 rcondf {2} 1. progress. skip. smt.
 skip. progress.
 unroll {1} 1.
 if. progress.  
-rcondf {1} 4. progress.
-wp. rnd. rnd. skip. progress. smt.
-wp. rnd. rnd. skip. progress. 
+rcondf {1} 3. progress.
+wp. rnd. skip. progress. smt.
+wp. rnd. skip. progress. 
 rcondf {1} 1. progress. skip. progress.
 qed.
 
 
-lemma whp_split_if_end' s e b r p P :  
-  (phoare [ M.whp_if_end : arg = (s,e,b,r) ==> P res ] = p)
-   => phoare [ M.whp : arg = (s,e+1,b,r) ==> P res ] = p.
+lemma whp_split_if_end' s e r p P :  
+  (phoare [ M.whp_if_end : arg = (s,e,r) ==> P res ] = p)
+   => phoare [ M.whp : arg = (s,e+1,r) ==> P res ] = p.
 proof. progress. bypr.
 progress.
-have <-: Pr[M.whp_if_end(s{m}, e{m}, b{m}, r{m}) @ &m : P res] = p.
-byphoare (_: arg = (s{m}, e{m}, b{m}, r{m}) ==> _).
+have <-: Pr[M.whp_if_end(s{m}, e{m}, r{m}) @ &m : P res] = p.
+byphoare (_: arg = (s{m}, e{m}, r{m}) ==> _).
 conseq H. auto. auto. byequiv.
 conseq whp_split_if_end. smt. auto. auto. auto.
 qed.
@@ -69,55 +72,87 @@ lemma lll (b a c : real) : a <= b => b <= c => a <= c.
 smt. qed.
 
     
-lemma whp_split_if_end_le s e b r p P :  
-  (phoare [ M.whp_if_end : arg = (s,e,b,r) ==> P res ] <= p)
-   => phoare [ M.whp : arg = (s,e+1,b,r) ==> P res ] <= p.
+lemma whp_split_if_end_le s e r p P :  
+  (phoare [ M.whp_if_end : arg = (s,e,r) ==> P res ] <= p)
+   => phoare [ M.whp : arg = (s,e+1,r) ==> P res ] <= p.
 proof. progress. bypr.
 progress.
-have zz : Pr[M.whp_if_end(s{m}, e{m}, b{m}, r{m}) @ &m : P res] <= p.
-byphoare (_: arg = (s{m}, e{m}, b{m}, r{m}) ==> _).
+have zz : Pr[M.whp_if_end(s{m}, e{m}, r{m}) @ &m : P res] <= p.
+byphoare (_: arg = (s{m}, e{m}, r{m}) ==> _).
 conseq H. auto. auto. 
-apply (lll Pr[M.whp_if_end(s, e, b, r) @ &m : P res] ).
+apply (lll Pr[M.whp_if_end(s, e, r) @ &m : P res] ).
 byequiv.
  conseq whp_split_if_end. smt. auto. auto. auto. apply zz.
 qed.
 
 
 
-lemma asdsad r:  forall e, 0 <= e =>
-  phoare[ M.whp_if_end : arg = (1,e,false,r) ==> !res.`2 ] = ((1%r/2%r) ^ (e+1)).
-proof. apply ge0ind. smt.
+lemma asdsad r:  MyP r = false => forall e, 0 <= e => 
+  phoare[ M.whp_if_end : arg = (1,e,r) ==> !MyP res ] = ((1%r/2%r) ^ (e+1)).
+proof. move => ipr. apply ge0ind. smt.
 progress. simplify.
   progress. proc.
 inline*. sp.
 rcondf 1. skip. smt.
 sp. 
-rcondt 1. skip. progress. wp.
-conseq (_: true ==> !b). 
-swap 1 1.  rnd. 
-conseq (_: true ==> !b). admit.
-rnd. skip. smt.
-progress. proc.
-  have phf: phoare[ M.whp : arg = (1, n+1, false, r) ==> ! res.`2] = (inv 2%r ^(n+1)).
- apply (whp_split_if_end' 1 n false r ((inv 2%r)^(n+1)) (fun (x : int * bool) => !x.`2) (H0 H) ).
-seq 1 : (!b) (inv 2%r ^(n+1)) (1%r/2%r) 1%r 0%r (!b => M.c <= e + 1).
-inline*. sp.  wp. while (e = e0 /\ (!b0 => M.c <= e + 1)).
-wp. rnd. rnd. skip. progress. smt. skip. progress. smt.
-call phf. skip.  auto.
 rcondt 1. skip. progress. smt.
-wp. simplify.  swap 1 1.  rnd. 
-conseq (_: _ ==> !b). progress. admit.
-rnd. skip. progress.
-smt.
+swap 1 1.  rnd.  simplify.
+wp.  skip.  progress. admit.
+progress. proc.
+  have phf: phoare[ M.whp : arg = (1, n+1, r) ==> !MyP res] = (inv 2%r ^(n+1)).
+ apply (whp_split_if_end' 1 n r ((inv 2%r)^(n+1)) (fun x => !MyP x) (H0 H) ).
+seq 1 : (!MyP ri) (inv 2%r ^(n+1)) (1%r/2%r) 1%r 0%r (!MyP ri => M.c <= e + 1).
+inline*. sp.
+seq 1 :  (!MyP r0 => M.c <= e + 1).
+ while (e = e0 /\ (!MyP r0 => M.c <= e0 + 1)).
+wp. 
+rnd.  skip. progress. smt. skip. progress. smt. sp.  skip. progress. 
+ call phf. skip.  auto.
+rcondt 1. skip. progress. smt.
+wp. simplify.  rnd.  simplify.
+skip. progress.
+admit.
 hoare. 
 rcondf 1. skip.  progress.  smt.
 simplify. skip. auto. smt.
 qed.
 
 
-lemma asdsadq r:  forall e, 0 <= e =>
-  phoare[ M.whp : arg = (1,e+1,false,r) ==> !res.`2 ] = ((1%r/2%r) ^ (e+1)).
+lemma asdsad_le r:  MyP r = false => forall e, 0 <= e => 
+  phoare[ M.whp_if_end : arg = (1,e,r) ==> !MyP res ]
+     <= ((1%r/2%r) ^ (e+1)).
+proof. move => ipr. apply ge0ind. smt.
+progress. simplify.
+  progress. proc.
+inline*. sp.
+rcondf 1. skip. smt.
+sp. 
+rcondt 1. skip. progress. smt.
+swap 1 1.  rnd.  simplify.
+wp.  skip.  progress. admit.
+progress. proc.
+  have phf: phoare[ M.whp : arg = (1, n+1, r) ==> !MyP res] <= (inv 2%r ^(n+1)).
+ apply (whp_split_if_end_le 1 n r ((inv 2%r)^(n+1)) (fun x => !MyP x) (H0 H) ).
+seq 1 : (!MyP ri) (inv 2%r ^(n+1)) (1%r/2%r) 1%r 0%r (!MyP ri => M.c <= e + 1).
+inline*. sp.
+seq 1 :  (!MyP r0 => M.c <= e + 1).
+ while (e = e0 /\ (!MyP r0 => M.c <= e0 + 1)).
+wp. 
+rnd.  skip. progress. smt. skip. progress. smt. sp.  skip. progress. 
+ call phf. skip.  auto.
+rcondt 1. skip. progress. smt.
+wp. simplify.  rnd.  simplify.
+skip. progress.
+admit.
+hoare. 
+rcondf 1. skip.  progress.  smt.
+simplify. skip. auto. smt.
+qed.
+
+
+lemma asdsadq r:  MyP r = false => forall e, 0 <= e =>
+  phoare[ M.whp : arg = (1,e+1,r) ==> !MyP res ] = ((1%r/2%r) ^ (e+1)).
 progress.
-have fact1  : phoare[ M.whp_if_end : arg = (1,e,false,r) ==> !res.`2 ] = ((1%r/2%r) ^ (e+1)). apply asdsad. auto.
- apply (whp_split_if_end' 1 (e) false r ((inv 2%r)^(e+1)) (fun (x : int * bool) => !x.`2)  fact1 ).
+have fact1  : phoare[ M.whp_if_end : arg = (1,e,r) ==> !MyP res ] = ((1%r/2%r) ^ (e+1)). apply (asdsad r H e H0). auto.
+ conseq (whp_split_if_end' 1 e r ((inv 2%r)^(e+1)) (fun x => !MyP x)  fact1 ).
 qed.
